src/Lustre/LClockSemantics.v
@@ -13,7 +13,7 @@ From Velus Require Import CommonList.
 From Velus Require Import Environment.
 From Velus Require Import Operators.
 From Velus Require Import Clocks.
-From Velus Require Import Lustre.LSyntax Lustre.LClocking Lustre.LOrdered Lustre.LSemantics.
+From Velus Require Import Lustre.LSyntax Lustre.LTyping Lustre.LClocking Lustre.LOrdered Lustre.LSemantics.
 From Velus Require Import CoindStreams.
 
 Local Set Warnings "-masking-absolute-name".
@@ -22,14 +22,16 @@ Module Type LCLOCKSEMANTICS
        (Import Op : OPERATORS)
        (Import OpAux : OPERATORS_AUX Op)
        (Import Syn : LSYNTAX Ids Op)
+       (Import Typ : LTYPING Ids Op Syn)
        (Import Clo : LCLOCKING Ids Op Syn)
        (Import Lord : LORDERED Ids Op Syn)
        (Import Str : COINDSTREAMS Op OpAux)
        (Import Sem : LSEMANTICS Ids Op OpAux Syn Lord Str).
 
-  Definition history_tl (H: history) : history := Env.map (@tl value) H.
+  Definition history_tl (H: history) : history :=
+    Env.map (@tl value) H.
 
-  Fact history_tl_find : forall (H: history) id vs,
+  Fact history_tl_find_Some : forall (H: history) id vs,
       Env.find id H = Some vs ->
       Env.find id (history_tl H) = Some (tl vs).
   Proof.
@@ -37,6 +39,17 @@ Module Type LCLOCKSEMANTICS
     unfold history_tl.
     rewrite Env.Props.P.F.map_o.
     rewrite Hfind. reflexivity.
+  Qed.
+
+  Fact history_tl_find_Some' : forall (H: history) id vs,
+      Env.find id (history_tl H) = Some vs ->
+      exists v, Env.find id H = Some (v ⋅ vs).
+  Proof.
+    intros H id vs Hfind.
+    unfold history_tl in Hfind.
+    rewrite Env.Props.P.F.map_o in Hfind.
+    apply option_map_inv_Some in Hfind as [vs' [Hfind Htl]]; subst.
+    exists (hd vs'). destruct vs'; auto.
   Qed.
 
   Fact history_tl_find_None : forall (H: history) id,
@@ -49,31 +62,289 @@ Module Type LCLOCKSEMANTICS
     rewrite Hfind. reflexivity.
   Qed.
 
-  CoInductive sem_clock: history -> Stream bool -> clock -> Stream bool -> Prop :=
-  | Sbase:
-      forall H b b',
-        b ≡ b' ->
-        sem_clock H b Cbase b'
-  | Son:
-      forall H b bk bs ck x k xs c,
-        sem_clock H b ck (true ⋅ bk) ->
-        sem_var H x (present c ⋅ xs) ->
-        val_to_bool c = Some k ->
-        sem_clock (history_tl H) (tl b) (Con ck x k) bs ->
-        sem_clock H b (Con ck x k) (true ⋅ bs)
-  | Son_abs1:
-      forall H b bk bs ck x k xs,
-        sem_clock H b ck (false ⋅ bk) ->
-        sem_var H x (absent ⋅ xs) ->
-        sem_clock (history_tl H) (tl b) (Con ck x k) bs ->
-        sem_clock H b (Con ck x k) (false ⋅ bs)
-  | Son_abs2:
-      forall H b bk bs ck x k c xs,
-        sem_clock H b ck (true ⋅ bk) ->
-        sem_var H x (present c ⋅ xs) ->
-        val_to_bool c = Some k ->
-        sem_clock (history_tl H) (tl b) (Con ck x (negb k)) bs ->
-        sem_clock H b (Con ck x (negb k)) (false ⋅ bs).
+  Fact history_tl_find_None' : forall (H: history) id,
+      Env.find id (history_tl H) = None ->
+      Env.find id H = None.
+  Proof.
+    intros H id Hfind.
+    unfold history_tl in Hfind.
+    rewrite Env.Props.P.F.map_o in Hfind.
+    apply option_map_inv_None in Hfind; auto.
+  Qed.
+
+  Definition env := Env.t value.
+
+  Definition history_nth (n : nat) (H: history) : env :=
+    Env.map (Str_nth n) H.
+
+  Definition history_hd (H: history) : env := history_nth 0 H.
+
+  Lemma history_nth_tl : forall H n,
+      history_nth (S n) H = history_nth n (history_tl H).
+  Proof.
+    intros H n.
+    unfold history_nth, history_tl.
+    rewrite Env.map_map. eapply Env.map_ext.
+    intros [x xs]. rewrite Str_nth_S; auto.
+  Qed.
+
+  Fact history_nth_find_Some : forall n (H: history) id vs,
+      Env.find id H = Some vs ->
+      Env.find id (history_nth n H) = Some (Str_nth n vs).
+  Proof.
+   induction n; intros H id vs Hfind.
+   - unfold history_nth.
+     rewrite Env.Props.P.F.map_o, Hfind. reflexivity.
+   - rewrite history_nth_tl.
+     rewrite IHn with (vs:=(tl vs)); auto.
+     erewrite history_tl_find_Some; auto.
+  Qed.
+
+  Fact history_nth_find_Some' : forall n (H: history) id v,
+      Env.find id (history_nth n H) = Some v ->
+      exists vs, Env.find id H = Some vs /\ vs # n = v.
+  Proof.
+   induction n; intros H id v Hfind.
+   - unfold history_nth in Hfind.
+     rewrite Env.Props.P.F.map_o in Hfind.
+     apply option_map_inv_Some in Hfind as [vs' [Hfind Heq]].
+     exists vs'; auto.
+   - rewrite history_nth_tl in Hfind.
+     apply IHn in Hfind as [vs' [Hfind Heq]].
+     apply history_tl_find_Some' in Hfind as [v' Hfind].
+     exists (v' ⋅ vs'); split; auto.
+  Qed.
+
+  Fact history_nth_find_None : forall n (H: history) id,
+      Env.find id H = None ->
+      Env.find id (history_nth n H) = None.
+  Proof.
+   induction n; intros H id Hfind.
+   - unfold history_nth.
+     rewrite Env.Props.P.F.map_o, Hfind. reflexivity.
+   - rewrite history_nth_tl.
+     rewrite IHn; auto.
+     erewrite history_tl_find_None; auto.
+  Qed.
+
+  Fact history_nth_find_None' : forall n (H: history) id,
+      Env.find id (history_nth n H) = None ->
+      Env.find id H = None.
+  Proof.
+   induction n; intros H id Hfind.
+   - unfold history_nth in Hfind.
+     rewrite Env.Props.P.F.map_o in Hfind.
+     apply option_map_inv_None in Hfind; auto.
+   - rewrite history_nth_tl in Hfind.
+     apply IHn in Hfind.
+     apply history_tl_find_None' in Hfind; auto.
+  Qed.
+
+  (** *** Interpreter *)
+  Fixpoint interp_clock_instant R base ck : bool :=
+    match ck with
+    | Cbase => base
+    | Con ck id b =>
+      let b' := interp_clock_instant R base ck in
+      match Env.find id R with
+      | Some v => match v with
+                  | OpAux.present v =>
+                    match OpAux.val_to_bool v with
+                    | Some true => andb b b'
+                    | Some false => andb (negb b) b'
+                    | _ => false
+                    end
+                  | _ => false
+                  end
+      | None => false
+      end
+    end.
+
+  CoFixpoint interp_clock H base ck : Stream bool :=
+    match base with
+    | b ⋅ base =>
+      (interp_clock_instant (history_hd H) b ck) ⋅ (interp_clock (history_tl H) base ck)
+    end.
+
+  Fact interp_clock_Cons : forall H b bs ck,
+      interp_clock H (b ⋅ bs) ck ≡ (interp_clock_instant (history_hd H) b ck) ⋅ (interp_clock (history_tl H) bs ck).
+  Proof.
+    intros H b bs ck; simpl.
+    constructor; simpl; reflexivity.
+  Qed.
+
+  Lemma interp_clock_nth : forall n H base ck,
+      (interp_clock H base ck) # n = interp_clock_instant (history_nth n H) (base # n) ck.
+  Proof.
+    induction n; intros H [b base] ck; rewrite interp_clock_Cons; simpl.
+    - repeat rewrite Str_nth_0. reflexivity.
+    - repeat rewrite Str_nth_S.
+      rewrite IHn, <- history_nth_tl. reflexivity.
+  Qed.
+
+  Definition wt_value (ty : type) (v : value) :=
+    match v with
+    | absent => True
+    | present v => wt_val v ty
+    end.
+
+  Definition wt_env_val (R : env) (xty : ident * type) :=
+    match Env.find (fst xty) R with
+    | None => False
+    | Some v => wt_value (snd xty) v
+    end.
+
+  Definition wt_env (vars : list (ident * type)) (R : env) :=
+    Forall (wt_env_val R) vars.
+
+  Definition wt_hist_val (H : history) (xty : ident * type) :=
+    match Env.find (fst xty) H with
+    | None => False
+    | Some vs => SForall (wt_value (snd xty)) vs
+    end.
+
+  Definition wt_hist (vars : list (ident * type)) (H : history) :=
+    Forall (wt_hist_val H) vars.
+
+  Fact wt_hist_wt_env : forall vars hist,
+      wt_hist vars hist ->
+      forall n, wt_env vars (history_nth n hist).
+  Proof.
+    intros vars hist Hwt n.
+    unfold wt_hist, wt_env in *.
+    eapply Forall_impl; [|eauto]; clear Hwt.
+    intros [x ty] Hwt.
+    unfold wt_hist_val, wt_env_val in *; simpl in *.
+    destruct (Env.find x hist) eqn:Hfind; [|inv Hwt].
+    apply history_nth_find_Some with (n:=n) in Hfind; rewrite Hfind.
+    rewrite SForall_forall in Hwt; auto.
+  Qed.
+
+  Fact history_hd_refines : forall H H',
+      Env.refines eq H H' ->
+      Env.refines eq (history_hd H) (history_hd H').
+  Proof.
+    intros H H' Href x v Hfind.
+    eapply history_nth_find_Some' in Hfind as [vs' [Hfind Heq]].
+    exists v; split; auto.
+    eapply Href in Hfind as [vs'' [? Hfind]]; subst.
+    eapply history_nth_find_Some in Hfind; eauto.
+  Qed.
+
+  Fact history_tl_refines : forall H H',
+      Env.refines eq H H' ->
+      Env.refines eq (history_tl H) (history_tl H').
+  Proof.
+    intros H H' Href x vs Hfind.
+    eapply history_tl_find_Some' in Hfind as [v' Hfind].
+    eapply Href in Hfind as [vs' [Heq' Hfind']].
+    exists (tl vs').
+    apply history_tl_find_Some in Hfind'.
+    split; auto.
+    destruct vs'; simpl. inv Heq'; auto.
+  Qed.
+
+  Lemma history_nth_refines : forall H H',
+      Env.refines eq H H' ->
+      forall n, Env.refines eq (history_nth n H) (history_nth n H').
+  Proof.
+    intros H H' Href n; revert H H' Href.
+    induction n; intros.
+    - apply history_hd_refines, Href.
+    - repeat rewrite history_nth_tl.
+      apply IHn, history_tl_refines, Href.
+  Qed.
+
+  Fact history_nth_add : forall H n id vs,
+      Env.Equal (history_nth n (Env.add id vs H)) (Env.add id (vs # n) (history_nth n H)).
+  Proof.
+    intros H n id vs id'.
+    destruct Env.find eqn:Hfind; symmetry.
+    - eapply history_nth_find_Some' in Hfind as [vs' [? Hfind]]; subst.
+      destruct (ident_eqb id id') eqn:Heq.
+      + rewrite ident_eqb_eq in Heq; subst.
+        rewrite Env.gss in *.
+        inv H0. auto.
+      + rewrite ident_eqb_neq in Heq.
+        rewrite Env.gso in *; auto.
+        eapply history_nth_find_Some in H0; eauto.
+    - eapply history_nth_find_None' in Hfind.
+      destruct (ident_eqb id id') eqn:Heq.
+      + rewrite ident_eqb_eq in Heq; subst.
+        rewrite Env.gss in *. inv Hfind.
+      + rewrite ident_eqb_neq in Heq.
+        rewrite Env.gso in *; auto.
+        eapply history_nth_find_None; auto.
+  Qed.
+
+  Fact interp_clock_instant_refines : forall R R' vars ck base,
+      wt_env vars R ->
+      wt_clock vars ck ->
+      Env.refines eq R R' ->
+      interp_clock_instant R base ck = interp_clock_instant R' base ck.
+  Proof with eauto.
+    induction ck; intros * Henv Hck Href; simpl in *; inv Hck.
+    - reflexivity.
+    - specialize (IHck base Henv H4 Href).
+      unfold wt_env in Henv; rewrite Forall_forall in Henv.
+      eapply Henv in H2; unfold wt_env_val in H2; simpl in H2.
+      destruct (Env.find i R) eqn:Hfind.
+      + apply Href in Hfind as [v' [? Hfind]]; subst. rewrite Hfind.
+        destruct v'; [auto|].
+        destruct (val_to_bool v); auto. repeat rewrite IHck. reflexivity.
+      + inv H2.
+  Qed.
+
+  Lemma interp_clock_refines : forall H H' vars ck base,
+      wt_hist vars H ->
+      wt_clock vars ck ->
+      Env.refines eq H H' ->
+      interp_clock H base ck ≡ interp_clock H' base ck.
+  Proof with eauto.
+    intros * Hhist Hck Href.
+    eapply ntheq_eqst; intros n.
+    repeat rewrite interp_clock_nth.
+    eapply interp_clock_instant_refines...
+    - eapply wt_hist_wt_env...
+    - eapply history_nth_refines...
+  Qed.
+
+  Fact interp_clock_instant_add : forall R id v ck base,
+      ~Is_free_in_clock id ck ->
+      interp_clock_instant (Env.add id v R) base ck = interp_clock_instant R base ck.
+  Proof.
+    induction ck; intros base Hnin; simpl; auto.
+    rewrite Env.gso.
+    - destruct Env.find as [[|v']|]; auto.
+      destruct val_to_bool as [[|]|]; f_equal; auto.
+      1,2:rewrite IHck; auto.
+      1,2:intro contra; apply Hnin; constructor; auto.
+    - intro contra; subst. apply Hnin. constructor.
+  Qed.
+
+  Instance interp_clock_instant_Proper:
+    Proper (@Env.Equal value ==> @eq bool ==> @eq clock ==> @eq bool)
+           interp_clock_instant.
+  Proof.
+    intros H H' Hequal base' base ? ck' ck ?; subst.
+    induction ck; simpl; auto.
+    - destruct Env.find as [[|v]|] eqn:Hfind;
+        rewrite Hequal in Hfind; rewrite Hfind; auto.
+      rewrite IHck; auto.
+  Qed.
+
+  Lemma interp_clock_add : forall H id vs ck base,
+      ~Is_free_in_clock id ck ->
+      interp_clock (Env.add id vs H) base ck ≡ interp_clock H base ck.
+  Proof.
+    intros * Hisfree.
+    eapply ntheq_eqst; intros n.
+    repeat rewrite interp_clock_nth.
+    rewrite history_nth_add.
+    apply interp_clock_instant_add; auto.
+  Qed.
+
+  (** Synchronization (alignement ?) *)
 
   CoInductive synchronized: Stream value -> Stream bool -> Prop :=
   | synchro_present:
@@ -85,119 +356,39 @@ Module Type LCLOCKSEMANTICS
         synchronized vs bs ->
         synchronized (absent ⋅ vs) (false ⋅ bs).
 
-  Fixpoint interp_clock H b cl : Stream bool :=
-    match cl with
-    | Cbase => b
-    | Con cl id b' =>
-      let b := interp_clock H b cl in
-      match Env.find id H with
-      | Some v =>
-        map2 (fun b v => match v with
-                      | OpAux.present v =>
-                        match OpAux.val_to_bool v with
-                        | Some true => andb b b'
-                        | Some false => andb b (negb b')
-                        | _ => false
-                        end
-                      | _ => false
-                      end) b v
-      | None => b
-      end
-    end.
-
-
-  Fact interp_clock_hd : forall cl H b bs,
-      hd (interp_clock H (b ⋅ bs) cl) =
-         match cl with
-         | Cbase => b
-         | Con cl id b' =>
-           let b := hd (interp_clock H (b ⋅ bs) cl) in
-           match Env.find id H with
-           | Some v => match (hd v) with
-                      | present v => match (OpAux.val_to_bool v) with
-                                    | Some true => andb b b'
-                                    | Some false => andb b (negb b')
-                                    | _ => false
-                                    end
-                      | absent => false
-                      end
-           | None => b
-           end
-         end.
-  Proof.
-    induction cl; intros H b0 bs.
-    - reflexivity.
-    - destruct (Env.find i H) eqn:Hfind; simpl.
-      + rewrite Hfind.
-        rewrite <- map2_hd. reflexivity.
-      + simpl. rewrite Hfind. reflexivity.
-  Qed.
-
-  Fact interp_clock_tl : forall cl H bs,
-      tl (interp_clock H bs cl) ≡ interp_clock (history_tl H) (tl bs) cl.
-  Proof.
-    induction cl; intros H bs; simpl in *.
-    - reflexivity.
-    - destruct (Env.find i H) eqn:Hfind.
-      + apply history_tl_find in Hfind. rewrite Hfind.
-        rewrite <- map2_tl. rewrite IHcl. reflexivity.
-      + apply history_tl_find_None in Hfind. rewrite Hfind. auto.
-  Qed.
-
-  Lemma interp_clock_Cons : forall cl H b bs,
-      interp_clock H (b ⋅ bs) cl ≡ hd (interp_clock H (b ⋅ bs) cl) ⋅ (interp_clock (history_tl H) bs cl).
-  Proof.
-    intros cl H b bs.
-    constructor; simpl; auto.
-    symmetry. replace bs with (tl (b ⋅ bs)) at 1; auto.
-    rewrite interp_clock_tl. reflexivity.
-  Qed.
-
-  Fact interp_clock_sound_instant : forall cl H bs bs',
-      sem_clock H bs cl bs' ->
-      hd (interp_clock H bs cl) = hd bs'.
+  Lemma synchronized_spec : forall vs bs,
+      synchronized vs bs <->
+      (forall n, (exists v, bs # n = true /\ vs # n = present v)
+            \/ (bs # n = false /\ vs # n = absent)).
   Proof with eauto.
-    induction cl; intros H [b0 bs] bs' Hsem; inv Hsem.
-    - inv H1...
-    - eapply IHcl in H4.
-      rewrite interp_clock_hd; simpl.
-      inv H7. eapply Env.find_1 in H1. rewrite H1.
-      rewrite <- H2; simpl. rewrite H9; simpl. rewrite H4; simpl.
-      destruct b...
-    - rewrite interp_clock_hd; simpl.
-      inv H8. eapply Env.find_1 in H1. rewrite H1.
-      rewrite <- H2. reflexivity.
-    - eapply IHcl in H4.
-      rewrite interp_clock_hd; simpl.
-      inv H7. eapply Env.find_1 in H1. rewrite H1.
-      rewrite <- H2; simpl. rewrite H9; simpl. rewrite H4; simpl.
-      destruct k...
+    split.
+    - intros H n. revert vs bs H.
+      induction n; intros.
+      + inv H; repeat rewrite Str_nth_0.
+        * left. exists v...
+        * right...
+      + inv H; repeat rewrite Str_nth_S...
+    - revert vs bs.
+      cofix CoFix; intros * H.
+      unfold_Stv vs; unfold_Stv bs.
+      1,4:(specialize (H 0); repeat rewrite Str_nth_0 in H;
+           destruct H as [[? [? ?]]|[? ?]]; try congruence).
+      1,2:(constructor; cofix_step CoFix H).
   Qed.
 
-  Lemma interp_clock_sound : forall cl H bs bs',
-      sem_clock H bs cl bs' ->
-      interp_clock H bs cl ≡ bs'.
+  Lemma const_synchronized : forall bs c,
+      synchronized (const bs c) bs.
   Proof with eauto.
-    cofix interp_clock_sound.
-    intros cl H [b bs] [b' bs'] Hsem.
-    constructor; simpl.
-    - apply interp_clock_sound_instant in Hsem...
-    - inv Hsem.
-      + inv H1...
-      + rewrite interp_clock_tl...
-      + rewrite interp_clock_tl...
-      + rewrite interp_clock_tl...
-  Admitted.
+    intros bs c.
+    remember (const bs c) as vs.
+    rewrite synchronized_spec. intros n.
+    eapply eq_EqSt, const_spec with (n:=n) in Heqvs.
+    rewrite Heqvs; clear Heqvs.
+    destruct (bs # n).
+    - left. eexists...
+    - right...
+  Qed.
 
-  (* Lemma sem_exp_synchronized : forall G H b e vs, *)
-  (*     sem_exp G H b e vs -> *)
-  (*     Forall2 synchronized vs (List.map (interp_clock H b) (clockof e)). *)
-  (* Proof. *)
-  (*   induction e; intros vs Hsem; inv Hsem. *)
-  (*   - (* const *) *)
-  (*     repeat constructor. *)
-  (*     rewrite H4. *)
-  (* Qed. *)
 End LCLOCKSEMANTICS.
 
 
@@ -206,9 +397,10 @@ Module LClockSemanticsFun
        (Op : OPERATORS)
        (OpAux : OPERATORS_AUX Op)
        (Syn : LSYNTAX Ids Op)
+       (Typ : LTYPING Ids Op Syn)
        (Clo : LCLOCKING Ids Op Syn)
        (Lord : LORDERED Ids Op Syn)
        (Str : COINDSTREAMS Op OpAux)
-       (Sem : LSEMANTICS Ids Op OpAux Syn Lord Str) <: LCLOCKSEMANTICS Ids Op OpAux Syn Clo Lord Str Sem.
-  Include LCLOCKSEMANTICS Ids Op OpAux Syn Clo Lord Str Sem.
+       (Sem : LSEMANTICS Ids Op OpAux Syn Lord Str) <: LCLOCKSEMANTICS Ids Op OpAux Syn Typ Clo Lord Str Sem.
+  Include LCLOCKSEMANTICS Ids Op OpAux Syn Typ Clo Lord Str Sem.
 End LClockSemanticsFun.
